FreydSSA/Terminator/Extrinsic/Subst.lean
@@ -3,6 +3,11 @@ import FreydSSA.Term.Extrinsic.Subst
 
 variable {φ ν α} [Φ : InstSet φ (Ty α)] [Φc : CohInstSet φ (Ty α)]
 
+-- inductive InstSet.USubstL [Φ : InstSet φ (Ty α)] (σ : ν → UTm φ ν)
+--   : Ctx ν (Ty α) → LCtx ν κ (Ty α) → Type _
+--   | nil : USubstL σ Γ []
+--   | cons : USubst σ Γ Δ → USubstL σ Γ L → USubstL σ Γ (sorry :: L)
+
 -- def UTerminator.Wf.subst {Γ Δ Γ' : Ctx ν (Ty α)} {σ}
 --   {t : UTerminator φ ν κ}
 --   (hσ : Φ.USubst σ Γ' Γ) : t.Wf Γ L → (t.rewrite σ).Wf Γ' L
